If-conversion optimization
Extends the instruction selection pass with an if-conversion optimization:
some if/then/else statements are converted into "select" operations,
which in turn can be compiled down to branchless instruction sequences
if the target architecture supports them.

The statements that are converted are of the form

        if (cond) { x = a1; } else { x = a2; }
        if (cond) { x = a1; }
        if (cond) { /*skip*/; } else { x = a2; }

where a1, a2 are "safe" expressions, containing no operations that can
fail at run-time, such as memory loads or integer divisions.

A heuristic in backend/Selectionaux.ml controls when the optimization occurs,
depending on command-line flags and the complexity of the "then" and "else"
branches.

backend/Selection.v
@@ -26,7 +26,7 @@ Require String.
 Require Import Coqlib Maps.
 Require Import AST Errors Integers Globalenvs Switch.
 Require Cminor.
-Require Import Op CminorSel.
+Require Import Op CminorSel Cminortyping.
 Require Import SelectOp SplitLong SelectLong SelectDiv.
 Require Machregs.
 
@@ -41,6 +41,12 @@ Function condexpr_of_expr (e: expr) : condexpr :=
   | Econdition a b c => CEcondition a (condexpr_of_expr b) (condexpr_of_expr c)
   | Elet a b => CElet a (condexpr_of_expr b)
   | _ => CEcond (Ccompuimm Cne Int.zero) (e ::: Enil)
+  end.
+
+Function condition_of_expr (e: expr) : condition * exprlist :=
+  match e with
+  | Eop (Ocmp c) el => (c, el)
+  | _ => (Ccompuimm Cne Int.zero, e ::: Enil)
   end.
 
 (** Conversion of loads and stores *)
@@ -173,6 +179,10 @@ Fixpoint sel_exprlist (al: list Cminor.expr) : exprlist :=
   | a :: bl => Econs (sel_expr a) (sel_exprlist bl)
   end.
 
+Definition sel_select_opt (ty: typ) (arg1 arg2 arg3: Cminor.expr) : option expr :=
+  let (cond, args) := condition_of_expr (sel_expr arg1) in
+  SelectOp.select ty cond args (sel_expr arg2) (sel_expr arg3).
+
 (** Recognition of immediate calls and calls to built-in functions
     that should be inlined *)
 
@@ -267,9 +277,63 @@ Definition sel_switch_long :=
     (fun arg ofs => subl arg (longconst (Int64.repr ofs)))
     lowlong.
 
+(** "If conversion": conversion of certain if-then-else statements
+  into branchless conditional move instructions. *)
+
+(** Recognition of "then" and "else" statements that support if-conversion.
+  Basically we are interested in assignments to local variables [id = e].
+  However the front-end may have put [skip] statements around these
+  assignments. *)
+
+Inductive stmt_class : Type :=
+  | SCskip
+  | SCassign (id: ident) (a: Cminor.expr)
+  | SCother.
+
+Function classify_stmt (s: Cminor.stmt) : stmt_class :=
+  match s with
+  | Cminor.Sskip => SCskip
+  | Cminor.Sassign id a => SCassign id a
+  | Cminor.Sseq Cminor.Sskip s => classify_stmt s
+  | Cminor.Sseq s Cminor.Sskip => classify_stmt s
+  | _ => SCother
+  end.
+
+(** External heuristic to limit the amount of if-conversion performed.
+    Arguments are: the condition, the "then" and the "else" expressions,
+    and the type at which selection is done. *)
+
+Parameter if_conversion_heuristic:
+  Cminor.expr -> Cminor.expr -> Cminor.expr -> AST.typ -> bool.
+
+Definition if_conversion_base
+      (ki: known_idents) (env: typenv)
+      (cond: Cminor.expr) (id: ident) (ifso ifnot:  Cminor.expr) : option stmt :=
+  let ty := env id in
+  if is_known ki id
+  && safe_expr ki ifso && safe_expr ki ifnot
+  && if_conversion_heuristic cond ifso ifnot ty
+  then option_map
+         (fun sel => Sassign id sel)
+         (sel_select_opt ty cond ifso ifnot)
+  else None.
+
+Definition if_conversion
+      (ki: known_idents) (env: typenv)
+      (cond: Cminor.expr) (ifso ifnot: Cminor.stmt) : option stmt :=
+  match classify_stmt ifso, classify_stmt ifnot with
+  | SCskip, SCassign id a =>
+      if_conversion_base ki env cond id (Cminor.Evar id) a
+  | SCassign id a, SCskip =>
+      if_conversion_base ki env cond id a (Cminor.Evar id)
+  | SCassign id1 a1, SCassign id2 a2 =>
+      if ident_eq id1 id2 then if_conversion_base ki env cond id1 a1 a2 else None
+  | _, _ => None
+  end.
+
 (** Conversion from Cminor statements to Cminorsel statements. *)
 
-Fixpoint sel_stmt (s: Cminor.stmt) : res stmt :=
+Fixpoint sel_stmt (ki: known_idents) (env: typenv) (s: Cminor.stmt) : res stmt :=
   match s with
   | Cminor.Sskip => OK Sskip
   | Cminor.Sassign id e => OK (Sassign id (sel_expr e))
@@ -291,15 +355,19 @@ Fixpoint sel_stmt (s: Cminor.stmt) : res stmt :=
       | _            => Stailcall sg (inl _ (sel_expr fn)) (sel_exprlist args)
       end)
   | Cminor.Sseq s1 s2 =>
-      do s1' <- sel_stmt s1; do s2' <- sel_stmt s2;
+      do s1' <- sel_stmt ki env s1; do s2' <- sel_stmt ki env s2;
       OK (Sseq s1' s2')
   | Cminor.Sifthenelse e ifso ifnot =>
-      do ifso' <- sel_stmt ifso; do ifnot' <- sel_stmt ifnot;
-      OK (Sifthenelse (condexpr_of_expr (sel_expr e)) ifso' ifnot')
+      match if_conversion ki env e ifso ifnot with
+      | Some s => OK s
+      | None =>
+          do ifso' <- sel_stmt ki env ifso; do ifnot' <- sel_stmt ki env ifnot;
+          OK (Sifthenelse (condexpr_of_expr (sel_expr e)) ifso' ifnot')
+      end
   | Cminor.Sloop body =>
-      do body' <- sel_stmt body; OK (Sloop body')
+      do body' <- sel_stmt ki env body; OK (Sloop body')
   | Cminor.Sblock body =>
-      do body' <- sel_stmt body; OK (Sblock body')
+      do body' <- sel_stmt ki env body; OK (Sblock body')
   | Cminor.Sexit n => OK (Sexit n)
   | Cminor.Sswitch false e cases dfl =>
       let t := compile_switch Int.modulus dfl cases in
@@ -314,7 +382,7 @@ Fixpoint sel_stmt (s: Cminor.stmt) : res stmt :=
   | Cminor.Sreturn None => OK (Sreturn None)
   | Cminor.Sreturn (Some e) => OK (Sreturn (Some (sel_expr e)))
   | Cminor.Slabel lbl body =>
-      do body' <- sel_stmt body; OK (Slabel lbl body')
+      do body' <- sel_stmt ki env body; OK (Slabel lbl body')
   | Cminor.Sgoto lbl => OK (Sgoto lbl)
   end.
 
@@ -322,8 +390,15 @@ End SELECTION.
 
 (** Conversion of functions. *)
 
+Definition known_id (f: Cminor.function) : known_idents :=
+  let add (ki: known_idents) (id: ident) := PTree.set id tt ki in
+  List.fold_left add f.(Cminor.fn_vars)
+      (List.fold_left add f.(Cminor.fn_params) (PTree.empty unit)).
+
 Definition sel_function (dm: PTree.t globdef) (hf: helper_functions) (f: Cminor.function) : res function :=
-  do body' <- sel_stmt dm f.(Cminor.fn_body);
+  let ki := known_id f in
+  do env <- Cminortyping.type_function f;
+  do body' <- sel_stmt dm ki env f.(Cminor.fn_body);
   OK (mkfunction
         f.(Cminor.fn_sig)
         f.(Cminor.fn_params)
