extraction/extraction.v
@@ -72,6 +72,7 @@ Extract Constant Iteration.GenIter.iterate =>
 (* Selection *)
 
 Extract Constant Selection.compile_switch => "Switchaux.compile_switch".
+Extract Constant Selection.if_conversion_heuristic => "Selectionaux.if_conversion_heuristic".
 
 (* RTLgen *)
 Extract Constant RTLgen.more_likely => "RTLgenaux.more_likely".
